src/study/Nemonuri.Study.CSharpSyntaxRewriter2.Modifier2/Nemonuri.StratifiedNodes.Factories.NodeLists.fst
@@ -96,13 +96,13 @@ let replace_range #t
     (requires L.contains node node_list)
     (ensures fun _ -> true)
   =
-  //assume (Some? (N.try_get_first_index_of_predicate node_list (op_Equality node)));
+  assume (N.ISome? (N.try_get_first_index_of_predicate node_list (op_Equality node)));
   let N.ISome _ index = N.try_get_first_index_of_predicate node_list (op_Equality node) in
   replace_range_at node_list index inserting_node_list
 
 let replace #t
   (node_list:N.node_list t) 
-  (node:N.node t) //{ L.contains node node_list }
+  (node:N.node t{ L.contains node node_list }) //
   (inserting_node:N.node t)
   : Tot (N.node_list t)
   =
